Bdd/Evaluate.lean
@@ -6,7 +6,7 @@ namespace Evaluate
 
 public section
 
-def evaluate (O : OBdd n m) : Vector Bool n → Bool := fun I ↦
+def evaluate {n m} (O : OBdd n m) : Vector Bool n → Bool := fun I ↦
   match h : O.1.root with
   | .terminal b => b
   | .node j => if I[O.1.heap[j].var] then evaluate (O.high h) I else evaluate (O.low h) I
@@ -23,12 +23,14 @@ lemma evaluate_evaluate : evaluate O = OBdd.evaluate O := by
     simp only [Pointer.node.injEq, OBdd.evaluate_node, *]
 termination_by O
 
-lemma evaluate_terminal {O : OBdd n m} : O.1.root = .terminal b → evaluate O = Function.const _ b := by
+lemma evaluate_terminal {n m} {O : OBdd n m} {b} :
+    O.1.root = .terminal b → evaluate O = Function.const _ b := by
   rw [evaluate_evaluate]
   exact OBdd.evaluate_terminal
 
-lemma evaluate_node {O : OBdd n m} (h : O.1.root = .node j) :
-    evaluate O = fun I ↦ if I[O.1.heap[j].var] then evaluate (O.high h) I else evaluate (O.low h) I := by
+lemma evaluate_node {n m} {O : OBdd n m} {j} (h : O.1.root = .node j) :
+    evaluate O = fun I ↦
+      if I[O.1.heap[j].var] then evaluate (O.high h) I else evaluate (O.low h) I := by
   rw [evaluate_evaluate]
   rw [OBdd.evaluate_node' h]
   simp [evaluate_evaluate]
